\documentclass{article}

\usepackage{amsmath}
\usepackage{amssymb}

\begin{document}
	
\author{Logan Grosz}
\title{2nd Order, Linear, Homogeneous Differential Equations}
\date{\today}

\maketitle

\begin{abstract}
	Abstract goes here...
\end{abstract}

\section{Declarations}

$variable$; variable description; $variable\quad domain\quad and\quad range,\quad if\quad applicable$

\section{Rule}

Math in text mode... \( f(x) = \sum_{i=0}^{n} \frac{a_i}{1+x} \)\\

Display mode: \\
\[ f(x) = \sum_{i=0}^{n} \frac{a_i}{1+x} \]

\section{Pre-Derivation}
Anything that the derivation relies on goes here

\section{Derivation}

	\begin{gather*}
		a\,y''+b\,y'+c\,y=0\\
		\text{Where } a,b,y\in k
	\end{gather*}
	\begin{align*}
		\text{Let }y&=e^{m\,x}\\
		\implies y'&=m\,e^{m\,x}\\
		\implies y''&=m^2\,e^{m\,x}
	\end{align*}
	\begin{align*}
		a\,m^2\,e^{m\,x}+b\,m\,e^{m\,x}+c\,e^{m\,x}&=0 &\text{Substitution}\\
		e^{m\,x}(a\,m^2+b\,m+c)&=0 &\text{Distribution}
	\end{align*}
	\begin{gather*}
		\forall x(e^{m\,x})\neq 0\\
		\implies a\,m^2+b\,m+c=0
	\end{gather*}
	\begin{align*}
		m&=\dfrac{-b\pm\sqrt{b^2-4\,a\,c}}{2\,a} &\text{Quadratic Formula}\\
		&\text{Let }\Delta=b^2-4\,a\,c &\text{Discriminant}\\
	\end{align*}
	\begin{align*}
		&\text{Case 1: }\Delta>0\implies m_1,m_2\in \mathbb{R}\\
		&\text{Case 2: }\Delta=0\implies m_1=m_2=\dfrac{-b}{2\,a}\\
		&\text{Case 3: }\Delta<0\implies m_1,m_2\in \mathbb{C}\\
	\end{align*}
	\begin{equation*}
		y=c_1\,e^{m_1\,x}+c_2\,e^{m_2\,x}
	\end{equation*}
	\begin{gather*}
		\text{Note: Case 2}\implies y_2=y_1\int{\dfrac{e^{\int{P(x)dx}}}{{y_1}^2}dx}
	\end{gather*}

\section{Exempli Gratia}

Examples of important instances

\end{document}