\documentclass{article}

\usepackage{amsmath}
\usepackage{amssymb}

\begin{document}
	
\author{Logan Grosz}
\title{2nd Order, Linear, Homogeneous Differential Equations}
\date{\today}

\maketitle

\begin{abstract}
	Abstract goes here...
\end{abstract}

\section{Declarations}

$\Delta$; Discriminant of the quadratic formula; $variable\quad domain\quad and\quad range,\quad if\quad applicable$

\section{Rule}

$$a\,y''+b\,y'+c\,y=0$$
$$\implies a\,m^2+b\,m+c=0$$

	\begin{align}
		\Delta>0\implies&y=c_2\,e^{m_1x}+c_2\,e^{m_2x}\\
		\Delta=0\implies&y=c_2\,e^{m\,x}+c_2\,x\,e^{m\,x}\\
		\Delta<0\implies&y=c_1\,e^{\alpha x}cos(\beta x)+c_2\,e^{\alpha x}sin(\beta x)
	\end{align}
\\
\noindent Note: This method works for homogeneous linear equations of any order. Just need to find roots and substitute for $m$.
\section{Pre-Derivation}
Graphs of sine and cosine (for the sin x =sin-x and cos -x = -cos x)

\section{Derivation}
	\subsection{Solving the Differential Equation}
		\begin{gather*}
			a\,y''+b\,y'+c\,y=0\\
			\text{Where } a,b,y\in k
		\end{gather*}
		\begin{align*}
			\text{Let }y&=e^{m\,x}\\
			\implies y'&=m\,e^{m\,x}\\
			\implies y''&=m^2\,e^{m\,x}
		\end{align*}
		\begin{align*}
			a\,m^2\,e^{m\,x}+b\,m\,e^{m\,x}+c\,e^{m\,x}&=0 &\text{Substitution}\\
			e^{m\,x}(a\,m^2+b\,m+c)&=0 &\text{Distribution}
		\end{align*}
		\begin{gather*}
			\forall x(e^{m\,x})\neq 0\\
			\implies a\,m^2+b\,m+c=0
		\end{gather*}
		\begin{align*}
			m&=\dfrac{-b\pm\sqrt{b^2-4\,a\,c}}{2\,a} &\text{Quadratic Formula}\\
			&\text{Let }\Delta=b^2-4\,a\,c &\text{Discriminant}\\
		\end{align*}
		\begin{align*}
			&\text{Case 1: }\Delta>0\implies m_1,m_2\in\mathbb{R}\\
			&\text{Case 2: }\Delta=0\implies m_1=m_2=\dfrac{-b}{2\,a}\\
			&\text{Case 3: }\Delta<0\implies m_1,m_2\in\mathbb{C}\\
		\end{align*}
	\subsection{Cases 1 \& 2}
		General solution for cases 1 \& 2:
		\begin{equation*}
			y=c_1\,e^{m_1\,x}+c_2\,e^{m_2\,x}
		\end{equation*}
		\begin{gather*}
			\text{Note: Case 2}\implies y_2=y_1\int{\dfrac{e^{\int{P(x)dx}}}{{y_1}^2}dx}
		\end{gather*}
	\subsection{Case 3}
		\begin{gather*}
			m_1,m_2\in\mathbb{C}\\
			m_1=\alpha+i\,\beta\\
			m_2=\alpha-i\,\beta\\
		\end{gather*}
		\begin{align*}
			y(x)=&c_1\,e^{(\alpha+i\,\beta)x}+c_2\,e^{(\alpha-\,\beta)x}&\text{Complex-valued solutions}\\
			=&c_1\,e^{\alpha x+i\,\beta x}+c_2\,e^{\alpha x-\,\beta x}&\\
			=&c_1\,e^{\alpha x}\,e^{i\,\beta x}+c_2\,e^{\alpha x}\,e^{-\beta x}&\\
			e^{i\Theta}=&cos\,\Theta+i\,sin\,\Theta,\,\Theta\in\mathbb{R}&\text{Euler's Formula}\\
		\end{align*}
		\begin{align*}
		 \text{Let }&c_1=c_2=1\\
			\implies& e^{\alpha x}\,e^{\beta x}+e^{\alpha x}\,e^{-\beta x}\\
			=&e^{\alpha x}(cos(\beta x)+i\,sin(\beta x)+cos(\beta x)-i\,sin(\beta x))\\
			=&e^{\alpha x}(2\,cos(\beta x))\\
			\implies&y_1=e^{\alpha x}\,cos(\beta x)
		\end{align*}
		\begin{align*}
			\text{Let }&c_1=1\,c_2=-1\\
			\implies& e^{\alpha x}\,e^{\beta x}-e^{\alpha x}\,e^{-\beta x}\\
			=&e^{\alpha x}(cos(\beta x)+i\,sin(\beta x)-cos(\beta x)-i\,sin(-\beta x))\\
			=&e^{\alpha x}(cos(\beta x)+i\,sin(\beta x)-cos(\beta x)+i\,sin(\beta x))\\
			=&2\,i\,e^{\alpha x}sin(\beta x)\\
			\implies&y_2=c_2\,sin(\beta x)
		\end{align*}
		General solution for case 3:
		\begin{equation*}
			y=c_1\,e^{\alpha x}cos(\beta x)+c_2\,e^{\alpha x}sin(\beta x)
		\end{equation*}

\section{Exempli Gratia}

Examples of important instances

\end{document}