\documentclass{article}

\usepackage{amsmath}
\usepackage{amssymb}

\begin{document}
	
\author{Logan Grosz}
\title{Linear Differential Equations}
\date{\today}

\maketitle

\begin{abstract}
	Strategy works with first order, linear differential equations
\end{abstract}

\section{Declarations}

$variable$; variable description; $variable\quad domain\quad and\quad range,\quad if\quad applicable$

\section{Rule}

\begin{align*}
&\dfrac{dy}{dx}+p(x)y=f(x)\\
\implies&\dfrac{d}{dx}[\mu(x)y]=\mu(x)f(x)\\
\implies&y=\dfrac{\int\mu(x)f(x)}{\mu(x)}dx\\
&\text{Where }\mu(x)=e^{\int p(x)dx}
\end{align*}

\section{Pre-Derivation}
$$a_1(x)\dfrac{dy}{dx}+a_0(x)y=g(x)$$\\
Must first get equation into standard form, with the derivative of y alone...
$$\dfrac{dy}{dx}+\dfrac{a_0(x)}{a_1(x)}y=\dfrac{g(x)}{a_1(x)}$$\\
$$\text{Let }\dfrac{a_0(x)}{a_1(x)}=p(x),\dfrac{g(x)}{a_1(x)}=f(x)$$\\
$$\implies\dfrac{dy}{dx}+p(x)y=f(x)$$

\section{Derivation}

\begin{align*}
\dfrac{dy}{dx}+p(x)y&=f(x)\\
\mu(x)\dfrac{dy}{dx}+\mu(x)p(x)y&=\mu(x)f(x)\\\\
\text{Finding the integration coeffecient, }&\mu(x)...\\
\exists\mu(x)|\dfrac{d}{dx}[\mu(x)y]&=\mu(x)\dfrac{dy}{dx}+\mu(x)p(x)y\\
Product\,rule\,of\,derivatives...\\
\dfrac{d}{dx}[\mu(x)y]&=\mu(x)\dfrac{dy}{dx}+\dfrac{d}{dx}[\mu(x)]y\\
\implies\dfrac{d}{dx}[\mu(x)]y&=\mu(x)p(x)y\\
\dfrac{d}{dx}\mu(x)&=\mu(x)p(x)\\
\dfrac{1}{\mu(x)}\dfrac{d}{dx}\mu(x)=p(x)\\
\int\dfrac{1}{\mu(x)}\dfrac{d}{dx}\mu(x)dx=\int p(x)dx\\
substituion\implies \ln|\mu(x)|&=\int p(x)dx\\
\mu(x)=\pm e^{\int p(x)dx+C_0}\\
\mu(x)=\pm C_0e^{\int p(x)dx}\\
\text{Let }\pm C_0=C_1=1\\
\mu(x)&=e^{\int p(x)dx}\\\\
\dfrac{d}{dx}[\mu(x)y]&=\mu(x)f(x)\\
\int\dfrac{d}{dx}[\mu(x)y]dx&=\int\mu(x)f(x)dx\\
\mu(x)y&=\int\mu(x)f(x)dx\\
y&=\dfrac{\int\mu(x)f(x)}{\mu(x)}
\end{align*}

\section{Exempli Gratia}

Examples of important instances

\subsection{Transient and steady state solution}

\text{Get in standard form and indentify p(x)...}
\begin{align*}
y'+3x^2y&=x^2\\
\implies p(x)&=3x^2\\\\
\end{align*}
\text{Find the integrating factor...}\\
\begin{align*}
\text{We know, }\mu(x)&=e^{\int p(x)dx}\\
\implies\mu(x)&=e^{\int3x^2dx}=e^{x^3}\\\\
\end{align*}
\text{Multiply through by the integrating factor...}\\
\begin{align*}
e^{x^3}y'+e^{x^3}3x^2y&=e^{x^3}x^2\\
\end{align*}
\text{Apply the product rule of derivatives...}\\
\begin{align*}
e^{x^3}y'+e^{x^3}3x^2y&=\dfrac{d}{dx}[e^{x^3}y]\\
\implies\dfrac{d}{dx}[e^{x^3}y]&=e^{x^3}x^2\\
\end{align*}
\text{Integrate}\\
\begin{align*}
\int\dfrac{d}{dx}[e^{x^3}y]dx&=\int e^{x^3}x^2dx\\
e^{x^3}y&=\dfrac{e^{x^3}}{3}+C\\
\end{align*}
\text{Solve for y}\\
\begin{align*}
y&=\dfrac{1}{3}+C\,e^{x^{-3}}\\\\
\end{align*}
\begin{align*}
\dfrac{1}{3}\implies \text{Steady state solution}\\
C\,e^{x^{-3}}\implies \text{Transient (approaches zero)}
\end{align*}

\end{document}