\documentclass{article}

\usepackage{amsmath}
\usepackage{amssymb}

\begin{document}
	
\author{Logan Grosz}
\title{Separable Equations}
\date{\today}

\maketitle

\begin{abstract}
	Abstract goes here...
\end{abstract}

\section{Declarations}

$\frac{dy}{dx}\triangleq y'$; Differential and prime notation equivalence;\\
$p(y)=\frac{1}{h(y)}$;P is the reciprocal of H, for neatness' sake;

\section{Rule}
$$\dfrac{dy}{dx}=g(x)\,h(y)$$\\
$$\implies\int p(y)\,dy=\int g(x)\,dx$$

\section{Pre-Derivation}
This rule only holds true if a differential equation is of first order and holds the following form, that being the product of two functions, one of x and one of y. See below...\\

$$\dfrac{dy}{dx}=g(x)\,h(y)$$

\section{Derivation}

\begin{align*}
	\dfrac{dy}{dx}&=g(x)\,h(y)\\
	\dfrac{1}{h(y)}\dfrac{dx}{dy}&=g(x)\\
	\text{Let }p(y)&=\dfrac{1}{h(y)},\,h(y)\neq 0\\
	\therefore\dfrac{dy}{dx}p(y)&=g(x)\\\\
	\text{Assume }y&=\phi(x),\text{ the solution.}\\
	\dfrac{dy}{dx}&=\phi '(x)\\\\
	p(\phi(x))\phi '(x)&=g(x)\\
	\int p(\phi(x))\phi '(x)dx&=\int g(x) dx\\\\
	\text{But since }y&=\phi(x)\\
	\implies dy&=\phi '(x)dx\\\\
	\therefore \int p(y)\,dy&=\int g(x)\,dx
\end{align*}

\section{Exempli Gratia}

Examples of important instances

\end{document}