\documentclass{article}

\usepackage{amsmath}
\usepackage{amssymb}

\begin{document}
	
\author{Logan Grosz}
\title{Linear Differential Equations}
\date{\today}

\maketitle

\begin{abstract}
	Strategy works with first order, linear differential equations
\end{abstract}

\section{Declarations}

$variable$; variable description; $variable\quad domain\quad and\quad range,\quad if\quad applicable$

\section{Rule}

\begin{align*}
&\dfrac{dy}{dx}+p(x)y=f(x)\\
\implies&\dfrac{d}{dx}[\mu(x)y]=\mu(x)f(x)\\
\implies&y=\dfrac{\int\mu(x)f(x)}{\mu(x)}\\
&\text{Where }\mu(x)=e^{\int p(x)dx}
\end{align*}

\section{Pre-Derivation}
$$a_1(x)\dfrac{dy}{dx}+a_0(x)y=g(x)$$\\
Must first get equation into standard form, with the derivative of y alone...
$$\dfrac{dy}{dx}+\dfrac{a_0(x)}{a_1(x)}y=\dfrac{g(x)}{a_1(x)}$$\\
$$\text{Let }\dfrac{a_0(x)}{a_1(x)}=p(x),\dfrac{g(x)}{a_1(x)}=f(x)$$\\
$$\therefore\dfrac{dy}{dx}+p(x)y=f(x)$$

\section{Derivation}

\begin{align*}
\dfrac{dy}{dx}+p(x)y=f(x)\\
\mu(x)\dfrac{dy}{dx}+\mu(x)p(x)y=\mu(x)f(x)\\\\
\text{Finding the integration coeffecient, }\mu(x)...\\
\exists\mu(x)|\dfrac{d}{dx}[\mu(x)y]&=\mu(x)\dfrac{dy}{dx}+\mu(x)p(x)y\\
\dfrac{d}{dx}[\mu(x)y]&=\mu(x)\dfrac{dy}{dx}+\dfrac{d}{dx}[\mu(x)]y\\
\implies\dfrac{d}{dx}[\mu(x)]y&=\mu(x)p(x)y\\
\dfrac{d}{dx}\mu(x)&=\mu(x)p(x)\\
\dfrac{1}{\mu(x)}du&=p(x)dx\\
\int\dfrac{1}{\mu(x)}du&=\int p(x)dx\\
\implies \ln\mu(x)&=\int p(x)dx\\
\mu(x)&=e^{\int p(x)dx}\\\\
\dfrac{d}{dx}[\mu(x)y]=\mu(x)f(x)\\
\int\dfrac{d}{dx}[\mu(x)y]=\int\mu(x)f(x)\\
\mu(x)y=\int\mu(x)f(x)\\
y=\dfrac{\int\mu(x)f(x)}{\mu(x)}
\end{align*}

\section{Exempli Gratia}

Examples of important instances

\end{document}