\documentclass{article}

\usepackage{amsmath}
\usepackage{amsfonts}

\begin{document}
	
\author{Logan Grosz}
\title{Taylor Series}
\date{\today}

\maketitle

\begin{abstract}
	Abstract goes here...
\end{abstract}

\section{Declarations}

$a$; domain value of which the series is about;\\
$n$; term in series; $x \in \mathbb{Z^+}$\\
$f^n$; nth derivative of a function;$n\in\mathbb{Z^+}, f^0(a)=f(a)$

\section{Rule}

\begin{gather*}
\sum_{n = 0}^{\infty}f^n(a)\dfrac{x-a}{n!}^n\\
= f(a)+f'(a)(x-a)+f''(a)\dfrac{(x-a)^2}{2!}+f'''(a)\dfrac{(x-a)^3}{3!}+f^{\text{iv}}(a)\dfrac{(x-a)^4}{4!}\\
\vdots\\
+ f^{\text{n-1}}(a)\dfrac{(x-a)^{n-1}}{(n-1)!} + f^{\text{n}}(a)\dfrac{(x-a)^n}{n!}
\end{gather*}

\section{Pre-Derivation}
Anything that the derivation relies on goes here

\section{Derivation}

Derivation goes here

\section{Exempli Gratia}

\subsection{Taylor Series Expansion of $e^x$ about 0}

$\begin{array}{c c}
	\parbox[c]{0.5\textwidth}{
		\begin{gather*}
			f(x) = e^x\\
			f'(x) = e^x\\
			f''(x) = e^x\\
			f'''(x) = e^x\\
			f^{\text{iv}}(x) = e^x\\
			\vdots
		\end{gather*}}
	&
	\parbox[c]{0.5\textwidth}{
		\begin{gather*}
			f(0) = 1\\
			f'(0) = 1\\
			f''(0) = 1\\
			f'''(0) = 1\\
			f^{\text{iv}}(0) = 1\\
			\vdots
		\end{gather*}}
\end{array}$

\begin{align*}
	e^x &= \sum_{n = 0}^{\infty}\dfrac{x^n}{n!}\\
		&= 1+x+\dfrac{x^2}{2!}+\dfrac{x^3}{3!}+\dfrac{x^4}{!4}+\dots
\end{align*}

\subsection{Taylor Series Expansion of cos about 0}

$\begin{array}{c c}
	\parbox[c]{0.5\textwidth}{
	\begin{gather*}
		f(x) = \cos x\\
		f'(x) = -\sin x\\
		f''(x) = -\cos x\\
		f'''(x) = \sin x\\
		f^{\text{iv}}(x) = \cos x\\
		\vdots
	\end{gather*}}
&
	\parbox[c]{0.5\textwidth}{
	\begin{gather*}
		f(0) = 1\\
		f'(0) = 0\\
		f''(0) = -1\\
		f'''(0) = 0\\
		f^{\text{iv}}(0) = 1\\
		\vdots
	\end{gather*}}
\end{array}$

\begin{align*}
	\cos x &= \sum_{n=0}^{\infty}(-1)^n\dfrac{x^{2n}}{(2n)!}\\
		   &= 1 - \dfrac{x^2}{2!}+\dfrac{x^4}{4!}-\dfrac{x^6}{6!}+\dfrac{x^8}{8!}-\dots
\end{align*}

\subsection{Taylor Series Expansion of sin about 0}

$\begin{array}{c c}
	\parbox[c]{0.5\textwidth}{
	\begin{gather*}
		f(x) = \sin x\\
		f'(x) = \cos x\\
		f''(x) = -\sin x\\
		f'''(x) = -\cos x\\
		f^{\text{iv}}(x) = \sin x\\
		\vdots
	\end{gather*}}
&
	\parbox[c]{0.5\textwidth}{
	\begin{gather*}
		f(0) = 0\\
		f'(0) = 1\\
		f''(0) = 0\\
		f'''(0) = -1\\
		f^{\text{iv}}(0) = 0\\
		\vdots
	\end{gather*}}
\end{array}$

\begin{align*}
	\sin x &= \sum{n=0}^{\infty}(-1)^n\dfrac{x^{2n+1}}{(2n+1)!}\\
		   &=
\end{align*}

\end{document}