\documentclass{article}

\usepackage{amsmath}
\usepackage{amssymb}

\begin{document}
	
\author{Logan Grosz}
\title{Journal Template}
\date{\today}

\maketitle

\begin{abstract}
	Abstract goes here...
\end{abstract}

\section{Declarations}

$variable$; variable description; $variable\quad domain\quad and\quad range,\quad if\quad applicable$

\section{Rule}

$$\dfrac{dy}{dx}+p(x)y=f(x)y^n,n\ne0\vee1$$\\
$$u=y^{1-n}$$\\

\section{Pre-Derivation}
Function must be of first order and in standard form...

$$\dfrac{dy}{dx}+p(x)y=f(x)y^n,n\ne0\vee1$$\\

\section{Derivation}

Derivation goes here

\section{Exempli Gratia}

\subsection{A basic problem...}

\begin{gather*}
\text{Get in standard form and find n}\\
\dfrac{dy}{dx}-\dfrac{3y}{2x}=\dfrac{2x}{y}\\
\implies n = -1\\\\
\text{Use rule to determine the substitive variable and its derivative}\\
\text{We know }u=y^{1-n}\text{, so } u=y^2\\
\implies y=u^{\frac{1}{2}}\\
\implies \dfrac{dy}{dx}=\dfrac{1}{2u^{\frac{1}{2}}}\dfrac{du}{dx}\\\\
\text{Substitute}\\
\dfrac{1}{2u^{\frac{1}{2}}}\dfrac{du}{dx}-\dfrac{3u^{\frac{1}{2}}}{2x}=\dfrac{2x}{u^{\frac{1}{2}}}\\\\
\text{Get to standard form of a 1st order linear equation.}\\
\dfrac{du}{dx}-\dfrac{3u}{x}=4x\\\\
\text{Solve differential equation with respect to }u\\
\text{We know, }\mu(x)=e^{\int p(x)dx}\\
\text{Let }p(x)=\dfrac{-3}{x}\\
\implies\mu(x)=e^{\int \frac{-3}{x}dx}=e^{-3\,ln(x)}=x^{-3}\\\\
\text{Multiple by }\mu(x)
\dfrac{du}{dx}x^{-3}-3ux^{-4}=4x^{-2}\\\\
\text{Apply product rule}\\
\dfrac{d}{dx}[x^{-3}u]=4x^{-2}\\\\
\text{Integrate}\\
\int\dfrac{d}{dx}[x^{-3}u]dx=\int 4x^{-2}dx\\
x^{-3}u=\dfrac{-4}{x}+C\\
u=-4x^2+C\,x^3\\\\
\text{Substitute in for }u\\
y^2=-4x^2+C\,x^3
\end{gather*}

\end{document}